# Proof of the quadratic formula
1. $ax^2 + bx + c = 0$  
(the a quadratic polynomial)

2. $x^2 + \frac{b}{a}x + \frac{c}{a} = 0 $  
(dividing by $a$)

3. $(x + \frac{b}{2a})^2 - \frac{b^2}{4a^2} + \frac{c}{a} = 0$  
(completeing the square)

4. $(x + \frac{b}{2a})^2 = \frac{b^2}{4a^2} - \frac{c}{a}$  
(rearranging)

5. $(x + \frac{b}{2a})^2 = \frac{b^2 -4ac}{4a^2}$  
(group terms)

6. $x + \frac{b}{2a} = \frac{\pm\sqrt{b^2 -4ac}}{2a}$  
(square root)

7. $x  = \frac{-b}{2a} \pm \frac{\sqrt{b^2 -4ac}}{2a}$  
(rearrange to make $x$ the subject)

8. $x = \frac{-b\pm\sqrt{b^2 - 4ac}}{2a}$  
(the quadratic formula)